tokeneer/token.dfy
@@ -1,18 +1,20 @@
-datatype clearanceLevel = Low | Medium | High
 
 class Token {
 
+
+
+
     var valifyer : bool;
-	var clearance_level : clearanceLevel;
-	var user_ID	: int;
+	var clearance_level : nat;
+	var user_ID	: nat;
+	
 	
 
-
-method INIT (id : int, sec_lvl : clearanceLevel)
+method INIT (id : nat, sec_lvl : nat)
 modifies this`valifyer
 modifies this`user_ID
 modifies this`clearance_level
-requires id >= 0 	// users always a positive integer
+requires 1 <= sec_lvl <= 3
 ensures 		valifyer 
 			&&  user_ID == id 
 			&&  clearance_level == sec_lvl
@@ -29,52 +31,52 @@ requires : that this current token already is valid
 ensures  : that the current token is invalid
 */
 
+
+
 method invalidateToken()
 modifies this`valifyer
 requires  valifyer
 ensures  !valifyer 
-{
 
+{
 valifyer := false;
 }
 
 }
 
 
-
-
 //================================= Class User  ===========================================
-
+/*
 
 class User{
 	var token 		: Token
 
-	method INIT()
+	method INIT(cl : ClearanceLevel)
+	
 	modifies this`token
 	ensures token == null	
 	{
 		token := null;
-
+		
 	}
 
 
 	}
 
-
+	*/
 //================================= Class Enrolmmentsys  ===========================================
 
 
-class EnrollmentSystem{
+class EnrollmentStation{
 
-var idCounter : int;
-var userSet : set<int>;
+var idCounter : nat;
+var userSet : set<nat>;
 
 predicate Valid_Enrollment()
 reads this`idCounter
 reads this`userSet
 {
 	 0 <= idCounter 
-
 }
 
 
@@ -82,25 +84,25 @@ method INIT()
 	modifies this`idCounter
 	modifies this`userSet
 		ensures userSet == {} && |userSet| == 0 
-		ensures idCounter == 0 
+		ensures idCounter == 0
   {
     userSet := {};
     idCounter := 0;
   }
 
-method register(user : User, cl : clearanceLevel)
+method register(cl : nat) returns (token : Token)
 	modifies this`userSet
 	modifies this`idCounter
-	modifies user`token, user.token
-		requires user != null
+		
 		requires 	Valid_Enrollment()
+		requires  1 <= cl <= 3
 		ensures 	Valid_Enrollment()
+		ensures old(idCounter) in userSet
 		ensures old(idCounter)  == idCounter - 1 
 		{
 
 			userSet := userSet + {idCounter};
-			// write method for this
-			user.token  := new Token.INIT(idCounter, cl);
+			token  := new Token.INIT(idCounter, cl);
 			idCounter := idCounter + 1;
 
 		}
@@ -108,9 +110,218 @@ method register(user : User, cl : clearanceLevel)
 
 
 
+}
+
+
+//================================= Class ID STATION  ===========================================
+
+/**
+There are three different types of ID one that validate to HIGH security, one to MEDIUM, one for LOW. It's decided in the 
+
+**/
+
+class IDStation{
+var authication_level : nat
+
+method INIT(auth_level : nat)
+	
+	modifies this`authication_level
+		requires  1 <= auth_level <= 3
+		ensures authication_level == auth_level
+			{
+	authication_level := auth_level;
+}
+
+
+
+/**
+ returns a bool that is connected to the supersystem, 
+
+ NOTE TO SUPERVISOR  : if the input token is null, then I wanted to invalidate the token, but I could not make it compile at all.
+ so instead I chose to change the design of the method to: e to require a non-null token from the user;
+ that is that the user ALREADY has enrolled to the system and recieved a valid token with a ID number
+
+ if isValid == true: user will be granted permission to enter the system
+			== false users token will be invalidated, alarm will sound and the doors too system will be shut.
+
+
+The input value of auth_level, will set the classes current level to that level via setClearanceLevel
+			CONDITIONS:
+
+				requires: a Natural number as ID
+				requires: a valid autication level
+				requires a nonnull token
+
+				ensures	: if userID != token.userID or token.clearanceLevel <=	auth_level					return false, invalidate token
+		:						returns false, invaldatetoken
+		:				token.clearanceLevel >=	auth_level													return true
+
+**/
+method openDoor(userID : nat, token : Token) returns (isAuthenticated : bool)
+	modifies this`authication_level
+	requires 1<= authication_level <=3
+    requires token != null
+		requires userID >= 0
+		ensures		(userID == token.user_ID) &&(token.clearance_level  >= authication_level )  <==> isAuthenticated
+{	
+
+	  isAuthenticated := (userID == token.user_ID) && token.clearance_level  >= authication_level ;
+  return isAuthenticated;
+  }
 
 }
 
+
+
+
+class TokeneerSystem {
+
+var doorOpen : bool;
+var alarmRing : bool;
+var idSt : IDStation;
+var enrollst: EnrollmentStation;
+
+predicate StationsRunning()
+	reads this.idSt;
+	reads this`idSt;
+	reads this.enrollst
+	reads this`enrollst;
+	
+	{
+	 idSt != null && enrollst != null 
+	}
+
+// tells us that the user can enroll and or apply for ID.
+predicate Applicable()
+	reads this`doorOpen;
+	reads this`alarmRing;
+{
+		!doorOpen && !alarmRing
+	}
+
+/*
+construct a fresh TokeneerSystem that 
+*/
+
+method INIT(cl : nat) 
+	modifies this`doorOpen
+	modifies this`alarmRing
+	modifies this.idSt	
+	modifies this`idSt
+	modifies this.enrollst
+	modifies this`enrollst
+	
+
+		requires 1 <= cl <= 3
+		ensures Applicable()
+		ensures StationsRunning()
+
+{
+	doorOpen := false;
+	alarmRing := false;
+	idSt := new IDStation.INIT(cl);
+	enrollst := new EnrollmentStation.INIT();
+
+}
+
+
+/**
+a user enrolls: it's token must either be null or not have a valid token
+
+**/
+
+method enroll ( cl : nat) returns (token : Token)
+modifies this.enrollst, this.enrollst`idCounter
+modifies this`enrollst
+
+	requires 1 <= cl <= 3
+	requires StationsRunning();
+
+	ensures StationsRunning()
+	ensures old(doorOpen) == doorOpen && old (alarmRing) == alarmRing
+{
+	token := enrollst.register(cl);
+}
+
+/*
+Checks that users token and opens the door if both userID and tokenID is the same, ASWELL as the current clearance level as the ID station.
+
+	requires a user that holds a token (that has enrolled) and is valid
+	and the comoponents of the system to be initaited
+
+	CONDITIONS 
+	-----------
+	ensures :	inputID == tokenID  
+				AND 
+				usersClearanceLevel	== enrollment then  :  openDoor = true , alarmRing = false
+
+				no alarm, and the door is open for the user
+
+
+				-------------
+	ensures:	inputID != tokenID
+				OR	
+				userClearanceLevel != enrollmentc			thne openDoor = false, alarmRing = true
+				door closes, alarm goes off
+
+
+*/
+method validateUser (id : nat, t : Token)
+modifies this`alarmRing
+modifies this`doorOpen
+modifies this.idSt, this`idSt
+modifies t
+modifies t`valifyer
+
+	requires StationsRunning()
+	requires 1 <= id <= 3
+	requires t != null
+	requires t.valifyer
+	requires idSt != null
+	requires 1 >= idSt.authication_level >= 3 	// setting the range for ClearanceLevel
+		
+		ensures StationsRunning()
+		ensures (old(t.user_ID) == id  && old(t.clearance_level) >= idSt.authication_level) ==> (!alarmRing && doorOpen)
+		ensures (old(t.user_ID) != id || old(t.clearance_level) <= old(idSt.authication_level)) <==> !doorOpen && !t.valifyer && alarmRing
+{
+		
+		//wanted to use method idStn.openDoor, but seems like that cant be done in dafny....
+		if (t.user_ID == id  && t.clearance_level >= idSt.authication_level){
+
+		alarmRing := false;
+		doorOpen := true;
+
+		}else {
+		alarmRing := true;
+		doorOpen := false;
+		t.invalidateToken();
+		
+		}
+}
+
+
+
+}
+
+
+
+
+
+
+
+class test{
+
+method Main(){
+
+var system := new TokeneerSystem.INIT(2);
+
+
+
+}
+
+
+
+}
 
 
 
